src/MachineImpl.v
@@ -26,191 +26,186 @@ Require Import Lia.
 Module MachineImpl : MachineSpec.
 
   Definition Word := MachineInt.
-(* Parameter Word *)
+  (* Parameter Word *)
 
-Definition wlt : Word -> Word -> bool := Z.ltb.
-(*  Parameter wlt : Word -> Word -> bool. *)
+  Definition wlt : Word -> Word -> bool := Z.ltb.
+  (*  Parameter wlt : Word -> Word -> bool. *)
 
-Definition weq : Word -> Word -> bool := Z.eqb.
-(* Parameter weq : Word -> Word -> bool. *)
+  Definition weq : Word -> Word -> bool := Z.eqb.
+  (* Parameter weq : Word -> Word -> bool. *)
 
-Definition WordEqDec : forall (w1 w2 : Word), {w1 = w2} + {w1 <> w2} := Z.eq_dec.
+  Definition WordEqDec : forall (w1 w2 : Word), {w1 = w2} + {w1 <> w2} := Z.eq_dec.
 
-Lemma weq_implies_eq :
+  Lemma weq_implies_eq :
     forall w1 w2,
       weq w1 w2 = true -> w1 = w2.
-  apply Z.eqb_eq.
-Qed.
+    apply Z.eqb_eq.
+  Qed.
 
-Lemma not_weq_implies_neq :
+  Lemma not_weq_implies_neq :
     forall w1 w2,
       weq w1 w2 = false -> w1 <> w2.
-Proof. 
-  intros w1 w2 HEqb HEq. unfold weq in *.
-  apply Z.eqb_eq in HEq.
-  rewrite HEq in HEqb.
-  congruence.
-Qed.
+  Proof. 
+    intros w1 w2 HEqb HEq. unfold weq in *.
+    apply Z.eqb_eq in HEq.
+    rewrite HEq in HEqb.
+    congruence.
+  Qed.
 
-Definition wle (w1 w2: Word) : bool :=
-  orb (wlt w1 w2) (weq w1 w2).
+  Definition wle (w1 w2: Word) : bool :=
+    orb (wlt w1 w2) (weq w1 w2).
+  
+  (*
+    Parameter wplus : Word -> nat -> Word.
+    Parameter wminus : Word -> nat -> Word.
+   *)
+  Definition wplus (w : Word) (n : nat) : Word :=
+    w + Z.of_nat n.
 
-(*
-Parameter wplus : Word -> nat -> Word.
-Parameter wminus : Word -> nat -> Word.
-*)  
-Definition wplus (w : Word) (n : nat) : Word :=
-  w + Z.of_nat n.
+  Lemma wplus_neq : forall w (n : nat),
+      (n > O)%nat -> w <> wplus w n.
+  Proof.
+    intros w n H Contra.
+    unfold wplus in *.
+    lia.
+  Qed.
 
-Lemma wplus_neq : forall w (n : nat),
-    (n > O)%nat -> w <> wplus w n.
-Proof.
-  intros w n H Contra.
-  unfold wplus in *.
-  lia.
-Qed.
+  Definition wminus (w : Word) (n : nat) : Word :=
+    w - Z.of_nat n.
 
-Definition wminus (w : Word) (n : nat) : Word :=
-  w - Z.of_nat n.
+  Definition Addr : Type := Word.
+  
+  Definition Register : Type := Word.
 
-Definition Addr : Type := Word.
+  Definition SP := 2.
+  Definition regEq : Register -> Register -> bool := Z.eqb.
 
-Definition Register : Type := Word.
+  Inductive Component:=
+  | Mem (a:Addr)
+  | Reg (r:Register)
+  | PC.
 
-Definition SP := 2.
-Definition regEq : Register -> Register -> bool := Z.eqb.
+  Definition keqb (k1 k2 : Component) : bool :=
+    match k1, k2 with
+    | Mem a1, Mem a2 => Z.eqb a1 a2
+    | Reg r1, Reg r2 => regEq r1 r2
+    | PC, PC => true
+    | _, _ => false
+    end.
 
-Inductive Component:=
-| Mem (a:Addr)
-| Reg (r:Register)
-| PC.
+  Axiom keqb_implies_eq :
+    forall k1 k2,
+      keqb k1 k2 = true -> k1 = k2.
+  Axiom not_keqb_implies_neq :
+    forall k1 k2,
+      keqb k1 k2 = false -> k1 <> k2.
 
-Definition keqb (k1 k2 : Component) : bool :=
-  match k1, k2 with
-  | Mem a1, Mem a2 => Z.eqb a1 a2
-  | Reg r1, Reg r2 => regEq r1 r2
-  | PC, PC => true
-  | _, _ => false
-  end.
+  (* A Value is a Word. *)
+  Definition Value : Type := Word.
 
-Axiom keqb_implies_eq :
-  forall k1 k2,
-    keqb k1 k2 = true -> k1 = k2.
-Axiom not_keqb_implies_neq :
-  forall k1 k2,
-    keqb k1 k2 = false -> k1 <> k2.
+  (* We use a risc-v machine as our machine state and a view as a map from its
+     components to their values. *)
+  Definition MachineState := RiscvMachine.
+  Definition View := Component -> Value.
 
-(* A Value is a Word. *)
-Definition Value : Type := Word.
+  (* Project what we care about from the RiscV state. *)
+  Definition proj (m:  MachineState) (k: Component):  Value :=
+    match k with
+    | Mem a =>
+      match (Spec.Machine.loadWord Spec.Machine.Execute (word.of_Z a)) m with
+      | (Some w, _) => regToZ_signed (int32ToReg w)
+      | (_, _) => 0
+      end
+    | Reg r =>
+      match (Spec.Machine.getRegister r) m with
+      | (Some w, _) => word.signed w
+      | (_, _) => 0
+      end
+    | PC =>
+      match (Spec.Machine.getPC) m with
+      | (Some w, _) => word.signed w
+      | (_, _) => 0
+      end
+    end.
 
-(* A Machine State is just a map from Components to Values. *)
+  (* Observations are values, or silent (tau) *)
+  Inductive Observation : Type := 
+  | Out (w:Value) 
+  | Tau. 
 
-Definition MachineState := RiscvMachine.
-Definition View := Component -> Value.
-
-(* Project what we care about from the RiscV state. *)
-Definition proj (m:  MachineState) (k: Component):  Value :=
-  match k with
-  | Mem a =>
-    match (Spec.Machine.loadWord Spec.Machine.Execute (word.of_Z a)) m with
-    | (Some w, _) => regToZ_signed (int32ToReg w)
-    | (_, _) => 0
+  (* A Machine State can step to a new Machine State plus an Observation. *)
+  Definition step (m : RiscvMachine) : RiscvMachine * Observation :=
+    (* returns option unit * state *)
+    (* TODO: What's an observation? *)
+    match Run.run1 RV32IM m with
+    | (_, s') => (s', Tau)
     end
-  | Reg r =>
-    match (Spec.Machine.getRegister r) m with
-    | (Some w, _) => word.signed w
-    | (_, _) => 0
-    end
-  | PC =>
-    match (Spec.Machine.getPC) m with
-    | (Some w, _) => word.signed w
-    | (_, _) => 0
-    end
-  end.
+  .
 
+  Definition FunID := nat.
+  Definition StackID := nat.
 
+  Definition EntryMap := Addr -> bool.
 
-(* Observations are values, or silent (tau) *)
-Inductive Observation : Type := 
-| Out (w:Value) 
-| Tau. 
+  Definition StackMap := Addr -> option StackID.
 
-(* A Machine State can step to a new Machine State plus an Observation. *)
-Definition step (m : RiscvMachine) : RiscvMachine * Observation :=
-  (* returns option unit * state *)
-  (* TODO: What's an observation? *)
-  match Run.run1 RV32IM m with
-  | (_, s') => (s', Tau)
-  end
-.
+  Inductive CodeAnnotation :=
+  | call
+  | ret
+  | yield
+  | share (f: MachineState -> Addr -> option bool)
+  | normal
+  .
 
-Definition FunID := nat.
-Definition StackID := nat.
+  Inductive CodeStatus :=
+  | inFun   : FunID -> CodeAnnotation -> CodeStatus
+  | notCode : CodeStatus
+  .
+  
+  Definition CodeMap := Addr -> CodeStatus.
 
-Definition EntryMap := Addr -> bool.
+  (* Stack ID of stack pointer *)
+  Definition activeStack (sm: StackMap) (m: MachineState) :
+    option StackID :=
+    sm (proj m (Reg SP)).
 
-Definition StackMap := Addr -> option StackID.
+  Definition stack_eqb : StackID -> StackID -> bool :=
+    Nat.eqb.
 
-Inductive CodeAnnotation :=
-| call
-| ret
-| yield
-| share (f: MachineState -> Addr -> option bool)
-| normal.
+  Definition optstack_eqb (o1 o2 : option StackID) : bool :=
+    match o1, o2 with
+    | Some n1, Some n2 => stack_eqb n1 n2
+    | None, None => true
+    | _, _ => false
+    end.
 
-Inductive CodeStatus :=
-| inFun   : FunID -> CodeAnnotation -> CodeStatus
-| notCode : CodeStatus.
+  Definition AnnotationOf (cdm : CodeMap) (a:Addr) : option CodeAnnotation :=
+    match cdm a with
+    | inFun f normal => None
+    | inFun f ann => Some ann
+    | notCode => None
+    end.
 
-Definition CodeMap := Addr -> CodeStatus.
+  Definition isCode' (cdm : CodeMap) (a:Addr) : bool :=
+    match cdm a with
+    | inFun _ _ => true
+    | notCode => false
+    end.
 
-(* Stack ID of stack pointer *)
-Definition activeStack (sm: StackMap) (m: MachineState) :
-  option StackID :=
-  sm (proj m (Reg SP)).
+  Definition justRet (mc m: MachineState) : Prop :=
+    proj m PC = wplus (proj mc PC) 4 /\ proj m (Reg SP) = proj mc (Reg SP).
 
-Definition stack_eqb : StackID -> StackID -> bool :=
-  Nat.eqb.
-
-Definition optstack_eqb (o1 o2 : option StackID) : bool :=
-  match o1, o2 with
-  | Some n1, Some n2 => stack_eqb n1 n2
-  | None, None => true
-  | _, _ => false
-  end.
-
-Definition AnnotationOf (cdm : CodeMap) (a:Addr) : option CodeAnnotation :=
-  match cdm a with
-  | inFun f normal => None
-  | inFun f ann => Some ann
-  | notCode => None
-  end.
-
-Definition isCode' (cdm : CodeMap) (a:Addr) : bool :=
-  match cdm a with
-  | inFun _ _ => true
-  | notCode => false
-  end.
-
-(*Definition isCall (cm: CallMap) (m: MachineState) (lay: Layout) : Prop :=
-  cm (m (Reg PC)) = Some lay.*)
-
-Definition justRet (mc m: MachineState) : Prop :=
-  proj m PC = wplus (proj mc PC) 4 /\ proj m (Reg SP) = proj mc (Reg SP).
-
-Definition justRet_dec mc m : {justRet mc m} + {~ justRet mc m}.
-Proof.
-  unfold justRet.
-  destruct (WordEqDec (proj m PC) (wplus (proj mc PC) 4));
-    destruct (WordEqDec (proj m (Reg SP)) (proj mc (Reg SP)));
-    try solve [left; auto];
-    right; intros [? ?]; auto.
-Qed.
+  Definition justRet_dec mc m : {justRet mc m} + {~ justRet mc m}.
+  Proof.
+    unfold justRet.
+    destruct (WordEqDec (proj m PC) (wplus (proj mc PC) 4));
+      destruct (WordEqDec (proj m (Reg SP)) (proj mc (Reg SP)));
+      try solve [left; auto];
+      right; intros [? ?]; auto.
+  Qed.
 
 (* TODO: More interesting state/abstract *)
 Definition PolicyState : Type := unit.
-(* TODO: Does this ever fail? *)
-(*Parameter initPolicyState : MachineState -> ProgramMap -> option PolicyState.*)
 
 (* TODO: Rename MPState to State and MPTrace to Trace, mp -> t *)
 Definition MPState : Type := MachineState * PolicyState.
@@ -228,21 +223,8 @@ Axiom mpstepCompat :
     mpstep (m,p) = Some (m',p',o) ->
     step m = (m',o).
 
-(* Confidentiality and Integrity Labels *)
-Inductive CLabel :=
-| HC
-| LC.
-
-Inductive ILabel :=
-| HI
-| LI.
-
-Definition Label := (CLabel * ILabel)%type.
-
-Definition Contour := Component -> Label.
-
-Definition integrityOf (l : Label) : ILabel := snd l.
-Definition confidentialityOf (l : Label) : CLabel := fst l.
+(* TODO: More interesting well-formedness condition *)
+Definition WFInitMPState (mp:MPState) := True.
 
 (********* Steps and Traces ***********)
 
@@ -300,136 +282,146 @@ Qed.
 
 (* ******************* Trace stuff ********************* *)
 
-(* We need to associate domainmaps with a trace. Here is some helpful machinery for associating
-   states in general with a trace. *)
 Section WITH_STATE.
-  Variable ContextState : Type.
-  Variable ContextStateUpdate : MachineState -> ContextState -> ContextState.
+  Variable CtxState : Type.
+  Variable CtxStateUpdate : MachineState -> CtxState -> CtxState.
+  Variable initCtx : CtxState.
   
-  Definition MCPState : Type := MachineState * ContextState * PolicyState.
-  Definition MCPTrace := TraceOf MCPState.
-  Definition mstate : MCPState -> MachineState := fun '(m,cs,p) => m.
-  Definition cstate : MCPState -> ContextState := fun '(m,cs,p) => cs.
-  Definition MCState : Type := MachineState * ContextState.
-  Definition MCTrace := TraceOf MCState.
-  Definition MPOTrace := MPTrace'.
+  Definition MPCState : Type := MachineState * PolicyState * CtxState.
+  Definition MPCTrace := TraceOf MPCState.
+  Definition mstate : MPCState -> MachineState := fun '(m,p,cs) => m.
+  Definition pstate : MPCState -> PolicyState := fun '(m,p,cs) => p.
+  Definition cstate : MPCState -> CtxState := fun '(m,p,cs) => cs.
 
-  (* WithContour relates an MPTrace to its MCPTrace given an initial contour state cs.
-     A finished trace (m,p) is related to (m,cs,p).
-     We relate a trace (notfinished (m,p) MP) to (notfinished (m,cs,p) MCP),
-     where MP relates to MCP given cs' produced by ContextStateUpdate. Additionally,
-     the relation requires that MP begin with m' and p' produced by mpstep (m,p),
-     so that only MPTraces produced by the step function relate to any MCPTrace *)
-  Inductive WithContextMP (cs:ContextState) : MPTrace -> MCPTrace -> Prop :=
-  | WCMPFinished : forall m p,
-      WithContextMP cs (finished (m,p)) (finished (m,cs,p))
-  | WCMPNotfinished : forall m p cs' m' p' o MP MCP,
-      mpstep (m,p) = Some (m',p',o) ->
-      ContextStateUpdate m cs = cs' ->
-      WithContextMP cs' MP MCP ->
-      head MP = (m',p') -> (* This checks that MP is actually real *)
-      WithContextMP cs (notfinished (m,p) MP) (notfinished (m,cs,p) MCP).
+  Definition mpcstep (mpc:MPCState) : option (MPCState * Observation) :=
+    option_map
+      (fun '(m,p,o) => (m,p,CtxStateUpdate m (cstate mpc),o))
+      (mpstep (mstate mpc,pstate mpc)).
+  
+  Inductive StepsTo : MPCState -> MPCState -> Prop :=
+  | already : forall mpc, StepsTo mpc mpc
+  | future : forall mpc mpc' mpc'' o,
+      StepsTo mpc mpc' ->
+      mpcstep mpc' = Some (mpc'',o) ->
+      StepsTo mpc mpc''.
 
-  Inductive WithContextM (cs:ContextState) : MTrace -> MCTrace -> Prop :=
-  | WCMFinished : forall m,
-      WithContextM cs (finished m) (finished (m,cs))
-  | WCMNotfinished : forall m cs' m' o MP MCP,
-      step m = (m',o) ->
-      ContextStateUpdate m cs = cs' ->
-      WithContextM cs' MP MCP ->
-      head MP = m' -> (* This checks that MP is actually real *)
-      WithContextM cs (notfinished m MP) (notfinished (m,cs) MCP).
+  Inductive StepsToWhenObs (P:MPCState -> Prop) : MPCState -> MPCState -> TraceOf Observation -> Prop :=
+  | when : forall mpc,
+      P mpc ->
+      StepsToWhenObs P mpc mpc (finished Tau)
+  | futureWhen : forall mpc mpc' mpc'' o O,
+      ~ P mpc ->
+      mpcstep mpc = Some (mpc',o) ->
+      StepsToWhenObs P mpc' mpc'' O ->
+      StepsToWhenObs P mpc mpc'' (notfinished o O).
 
+  Definition StepsToWhen P mpc mpc' := exists O, StepsToWhenObs P mpc mpc' O.
+
+  Inductive FullObsTrace : MPCState -> TraceOf Observation -> Prop :=
+  | stepIt : forall mpc mpc' o O,
+      mpcstep mpc = Some (mpc',o) ->
+      FullObsTrace mpc' O ->
+      FullObsTrace mpc (notfinished o O).
+
+  Definition NeverStepsToObs P mpc O :=
+    FullObsTrace mpc O /\
+    forall mpc',
+      ~ StepsToWhen P mpc mpc'.
+
+  Definition Reachable (mpc:MPCState) : Prop :=
+    exists mpinit,
+      WFInitMPState mpinit /\ StepsTo (mpinit,initCtx) mpc.
+
+  CoFixpoint MPCTraceOf (mpc : MPCState) : MPCTrace :=
+    match mpcstep mpc with
+    | None => finished mpc
+    | Some (mpc',o) => notfinished mpc (MPCTraceOf mpc')
+    end.
+
+  CoInductive MPCTraceToWhen (P:MPCState -> Prop) : MPCState -> MPCTrace -> Prop :=
+  | TTWNow : forall mpc,
+      P mpc ->
+      MPCTraceToWhen P mpc (finished mpc)
+  | TTWNever : forall mpc,
+      mpcstep mpc = None ->
+      MPCTraceToWhen P mpc (finished mpc)
+  | TTWLater : forall mpc mpc' o MPC,
+      ~ P mpc ->
+      mpcstep mpc = Some (mpc',o) ->
+      MPCTraceToWhen P mpc' MPC ->
+      MPCTraceToWhen P mpc (notfinished mpc MPC)
+  .
+  
   (* Similarly, with WithObs we relate an MCPTrace into the MPOTrace
      corresponding to its steps annotated with their observations. We feed
      each step's observation forward, to line up with the machine state that follows that step.
      We will need this later. *)
-  Inductive WithObs (o:Observation) : MCPTrace -> MPOTrace -> Prop :=
-  | WOFinished : forall m c p,
-      WithObs o (finished (m,c,p)) (finished (m,p,o))
-  | WONotfinished : forall m c p m' c' o' p' MP MPO,
-      WithObs o' MP MPO ->
-      mpstep (m,p) = Some ((m',p'),o) ->
-      head MP = (m',c',p') ->
-      WithObs o (notfinished (m,c,p) MP) (notfinished (m,p,o) MPO).
+  Inductive WithObs (o:Observation) : MPCTrace -> TraceOf Observation -> Prop :=
+  | WOFinished : forall mpc,
+      WithObs o (finished mpc) (finished o)
+  | WONotfinished : forall mpc mpc' o' MPC O,
+      WithObs o' MPC O ->
+      mpcstep mpc = Some (mpc',o') ->
+      WithObs o (notfinished mpc MPC) (notfinished o O).
   
   (* ObsOfMCP starts the observation with Tau, reflecting that initially
      there is no observation until a step occurs. *)
-  Definition ObsOfMCP := WithObs Tau.
-
-  Inductive WithObsM (o:Observation) : MCTrace -> TraceOf (MachineState*Observation) -> Prop :=
-  | WOMFinished : forall m c,
-      WithObsM o (finished (m,c)) (finished (m,o))
-  | WOMNotfinished : forall m c m' c' o' M MO,
-      WithObsM o' M MO ->
-      step m = (m',o) ->
-      head M = (m',c') ->
-      WithObsM o (notfinished (m,c) M) (notfinished (m,o) MO).
+  Definition ObsOfMPC := WithObs Tau.
   
-  (* ObsOfMCP starts the observation with Tau, reflecting that initially
-     there is no observation until a step occurs. *)
-  Definition ObsOfMC := WithObsM Tau.
-
-  (* ContextSegment relates two MCPTraces given a condition f on machine and context states,
-     where the second is a longest subtrace of the first such that f holds on all elements
-     except the final. So, it will always have at least two elements, and its head will have been
-     preceded by one on which f does not hold, while the last (if any) also does not have f hold.
-     
-     We will use this machinery to clip out sections of a trace that we want to check
-     against a property, with the final state reflecting the state after some relevant execution.
-   *)
-  Inductive ContextSegment (f : MachineState -> ContextState -> Prop) : MCPTrace -> MCPTrace -> Prop :=
-  | CSCurrent : forall MCP MCP' m cs p,
-      head MCP = (m,cs,p) ->
-      f m cs ->
-      PrefixUpTo (fun '(m,cs,p) => ~ f m cs) MCP MCP' ->
-      ContextSegment f (notfinished (m,cs,p) MCP) (notfinished (m,cs,p) MCP')
-  | CSNot : forall MCP MCPpre MCPsuff MCP' m cs p,
-      head MCP = (m,cs,p) ->
-      ~ f m cs ->
-        SplitInclusive (fun '(m,cs,p) => f m cs) MCP MCPpre MCPsuff ->
-        ContextSegment f MCPsuff MCP' ->
-        ContextSegment f MCP MCP'
-  | CSSkip : forall MCP MCPpre MCPsuff MCP' m cs p,
-      head MCP = (m,cs,p) ->
-      f m cs ->
-      SplitInclusive (fun '(m,cs,p) => f m cs) MCP MCPpre MCPsuff ->
-      ContextSegment f MCPsuff MCP' ->
-      ContextSegment f MCP MCP'
+  Inductive Segment (f : MPCState -> Prop) : MPCTrace -> MPCTrace -> Prop :=
+  | SegCurrent : forall MPC MPC' mpc,
+      f mpc ->
+      PrefixUpTo (fun mpc' => ~ f mpc') MPC MPC' ->
+      Segment f (notfinished mpc MPC) (notfinished mpc MPC')
+  | SegNot : forall MPC MPCpre MPCsuff MPC' mpc,
+      ~ f mpc ->
+      SplitInclusive f MPC MPCpre MPCsuff ->
+      Segment f MPCsuff MPC' ->
+      Segment f (notfinished mpc MPC) MPC'
+  | SegSkip : forall MPC MPCpre MPCsuff MPC' mpc,
+      f mpc ->
+      SplitInclusive f MPC MPCpre MPCsuff ->
+      Segment f MPCsuff MPC' ->
+      Segment f (notfinished mpc MPC) MPC'
   .
 
-  Inductive ContextSegmentM (f : MachineState -> ContextState -> Prop) : MCTrace -> MCTrace -> Prop :=
-  | CSMCurrent : forall MC MC' m cs,
-      head MC = (m,cs) ->
-      f m cs ->
-      PrefixUpTo (fun '(m,cs) => ~ f m cs) MC MC' ->
-      ContextSegmentM f (notfinished (m,cs) MC) (notfinished (m,cs) MC')
-  | CSMNot : forall MC MCpre MCsuff MC' m cs,
-      head MC = (m,cs) ->
-      ~ f m cs ->
-      SplitInclusive (fun '(m,cs) => f m cs) MC MCpre MCsuff ->
-      ContextSegmentM f MCsuff MC' ->
-      ContextSegmentM f MC MC'
-  | CSMSkip : forall MC MCpre MCsuff MC' m cs,
-      head MC = (m,cs) ->
-      f m cs ->
-      SplitInclusive (fun '(m,cs) => f m cs) MC MCpre MCsuff ->
-      ContextSegmentM f MCsuff MC' ->
-      ContextSegmentM f MC MC'
-  .
+  Definition ReachableSegment (f : MPCState -> Prop) (MPC:MPCTrace) : Prop :=
+    exists mpinit,
+      WFInitMPState mpinit /\ Segment f (MPCTraceOf (mpinit,initCtx)) MPC.
+
+  Lemma ReachableStepsToWhenSegment :
+    forall mpc mpc' P,
+      Reachable mpc ->
+      StepsToWhen P mpc mpc' ->
+      exists MPC,
+        ReachableSegment P MPC /\
+        head MPC = mpc /\
+        Last MPC mpc'.
+  Proof.
+  Admitted.
+(*    intros. destruct H0 as [O]. induction H0.
+    - exists (finished mpc).
+      split.
+      + unfold ReachableSegment.
+        unfold Reachable in H.
+        destruct H as [mpinit]; exists mpinit.
+        destruct H. split; auto. *)
+        
 
 End WITH_STATE.
 
-Arguments WithContextMP {_}  _ _ _ _.
-Arguments WithContextM {_}  _ _ _ _.
-Arguments ContextSegment {_} _ _ _.
-Arguments ContextSegmentM {_} _ _ _.
-Arguments ObsOfMCP {_}.
-Arguments ObsOfMC {_}.
-Arguments MCPState {_}.
-Arguments MCPTrace {_}.
+Arguments Segment {_} _ _ _.
+Arguments ObsOfMPC {_}.
+Arguments MPCState {_}.
+Arguments MPCTrace {_}.
 Arguments cstate {_}.
 Arguments mstate {_}.
-
+Arguments pstate {_}.
+Arguments Reachable {_} _ _ _.
+Arguments mpcstep {_} _ _.
+Arguments StepsToWhenObs {_} _ _ _ _.
+Arguments StepsToWhen {_} _ _ _.
+Arguments ReachableSegment {_} _ _ _.
+Arguments NeverStepsToObs {_} _ _ _.
 
 End MachineImpl.
